\subsection{Household Decision Rules}

From the household budget and preferences in Section \ref{subsec:hh}, households solve
\begin{alignat*}{4}
    \max_{\{c_{i, t}, \ell_{i, t}, b_{i, t}\}_{t = 0}^\infty} \quad & \E \sum_{t = 0}^\infty \beta^t \left[ \frac{c_{i, t}^{1 - \gamma}}{1 - \gamma} - \phi \frac{\ell_{i, t}^{1 + \chi}}{1 + \chi} \right] \\
    \text{subject to} \quad & b_{i, t} + c_{i, t} = R_t b_{i, t-1} + W_t z_{i, t} \ell_{i, t} + D_t + \eta_t - \tau_t^L z_{i, t}^{\tau_t^P} \\
    & b_{i, t} \geq \underline{b}.
\end{alignat*}
This gets the Lagrangian
\begin{align*}
    \mathcal{L} = \E \sum_{t = 0}^\infty \beta^t \Biggl[ \frac{c_{i, t}^{1 - \gamma}}{1 - \gamma} &- \phi \frac{\ell_{i, t}^{1 + \chi}}{1 + \chi} \\
     &+ \lambda_{i, t} \left( R_t b_{i, t-1} + W_t z_{i, t} \ell_{i, t} + D_t + \eta_t - \tau_t^L z_{i, t}^{\tau_t^P} - b_{i, t} - c_{i, t} \right) \notag \\
     &+ \mu_{i, t} \left(b_{i, t} - \underline{b} \right) \Biggr] \notag
\end{align*}
which has the FOCs
\begin{align*}
    \lambda_{i, t} &= c_{i, t}^{-\gamma} \\
    \lambda_{i, t} &= \frac{\phi}{W_t z_{i, t}} \ell_{i, t}^\chi \\
    \lambda_{i, t} &= \E \beta R_{t + 1} \lambda_{i, t+1} + \mu_{i, t}
\end{align*}
for consumption, labor, and bonds respectively. Combining the FOCs for consumption and labor gets the intratemporal constraint
\begin{equation*}
    c_{i, t}^{-\gamma} = \frac{\phi}{W_t z_{i, t}} \ell_{i, t}^\chi,
\end{equation*}
and combining the FOCs for consumption and bonds gets
\begin{equation*}
    c_{i, t}^{-\gamma} = \beta R_{t + 1} c_{i, t + 1}^{-\gamma} + \mu_{i, t}.
\end{equation*}
Since $\mu_{i, t} \geq 0$, this becomes the Euler Equation
\begin{equation*}
    c_{i, t}^{-\gamma} \geq \beta R_{t + 1} c_{i, t + 1}^{-\gamma}
\end{equation*}
which holds with equality whenever the borrowing constraint is not binding and $b_{i, t} > \underline{b}$.


\subsection{Final Goods Firm Conditions}

Final goods firms earn revenue $P_t Y_t$ and have costs $\int_0^1 y_{j, t} p_{j, t} dj$. Therefore, the profit maximization condition for firms is
\begin{equation*}
    \max_{y_{j, t}} \quad P_t Y_t - \int_0^1 p_{j, t} y_{j, t} dj.
\end{equation*}
Plugging in the aggregator, this becomes
\begin{equation*}
    \max_{y_{j, t}} \quad P_t \left( \int_0^1 y_{j, t}^\frac{1}{\psi_t} dj \right)^{\psi_t} - \int_0^1 p_{j, t} y_{j, t} dj
\end{equation*}
which has the FOC
\begin{equation*}
    p_{j, t} = P_t \left( \int_0^1 y_{j, t}^\frac{1}{\psi_t} dj \right)^{\psi_t - 1} y_{j, t}^\frac{1 - \psi_t}{\psi_t}.
\end{equation*}
Rearranging this gets
\begin{equation*}
    y_{j, t} = \left( \frac{p_{j, t}}{P_t} \right)^\frac{\psi_t}{1 - \psi_t} \left( \int_0^1 y_{j, t}^\frac{1}{\psi_t} dj \right)^{\psi_t} = Y_t \left( \frac{p_{j, t}}{P_t} \right)^\frac{\psi_t}{1 - \psi_t}   
\end{equation*}
which is the demand for intermediate good $j$. Plugging this back into the aggregator means
\begin{align*}
    Y_t &= \left( \int_0^1 \left(Y_t \left( \frac{p_{j, t}}{P_t} \right)^\frac{\psi_t}{1 - \psi_t}\right)^\frac{1}{\psi_t} dj \right)^{\psi_t} \\
    &= Y_t \frac{1}{P_t^\frac{\psi_t}{1 - \psi_t}} \left( \int_0^1 p_{j, t}^\frac{1}{1 - \psi_t} dj \right)^{\psi_t}.
\end{align*}
Rearranging this gets the price aggregator
\begin{equation*}
    P_t = \left(\int_0^1 p_{j, t}^\frac{1}{1 - \psi_t} dj \right)^{1 - \psi_t}.
\end{equation*}


\subsection{Philips Curve Derivation}

Intermediate goods firms pick prices to maximize expected discounted real profits solving
\begin{equation*}
    \max_{\{p_{j, t}\}_{t = 0}^\infty} \quad \E \sum_{s = t}^\infty R_{t, s}^{-1} \left[ \frac{p_{j, s}}{P_s} y_{j, s} - W_s n_{j, s} - m_{j, s} \right]
\end{equation*}
where $R_{t, s} = \prod_{q = t + 1}^s R_q$ represents the real gross return of bonds from period $t$ to $s$. Plugging in the demand function, production function, and adjustment costs gets
\begin{equation*}
    \max_{\{p_{j, t}\}_{t = 0}^\infty} \quad \E \sum_{s = t}^\infty R_{t, s}^{-1} Y_s \left(\frac{p_{j, s}}{P_s}\right)^\frac{1}{1 - \psi_t} \left[ \frac{p_{j, s}}{P_s} - \frac{W_s}{A_s} - \frac{\psi_s}{\psi_s - 1} \frac{1}{2 \kappa} \left(\frac{p_{j, s}}{{\overline{\pi} p_{j, s - 1}}} - 1\right)^2 \right]
\end{equation*}
This has the FOC with respect to $p_{j, t}$ of
\begin{align*}
    \frac{1}{2 \kappa} Y_t \left(\frac{p_{j, t}}{P_t}\right)^\frac{\psi_t}{1 - \psi_t} p_{j, t}^{-1} \left(\frac{p_{j, t}}{\overline{\pi} p_{j, t-1}} - 1\right)^2 + \frac{\psi_t}{\psi_t - 1} \frac{1}{\kappa} Y_t \left(\frac{p_{j, t}}{P_t}\right)^\frac{\psi_t}{1 - \psi_t} \frac{1}{\overline{\pi} p_{j, t-1}}\left(\frac{p_{j, t}}{\overline{\pi} p_{j, t-1}} - 1\right) \\
    = \frac{\psi_t}{\psi_t - 1} \frac{1}{\kappa} R_{t+1}^{-1} Y_{t+1} \left(\frac{p_{j, t}}{P_t}\right)^\frac{\psi_t}{1 - \psi_t} \frac{p_{j, t+1}}{\overline{\pi} p_{j, t}} p_{j, t}^{-1} \left(\frac{p_{j, t+1}}{\overline{\pi} p_{j, t}} - 1\right) \\
    + \frac{\psi_t}{\psi_t - 1} \left(\frac{p_{j, t}}{P_t}\right)^\frac{\psi_t}{1 - \psi_t} p_{j, t}^{-1} \frac{W_t}{A_t} - \frac{1}{\psi_t - 1} Y_t \left(\frac{p_{j, t}}{P_t}\right)^\frac{\psi_t}{1 - \psi_t} p_{j, t}^{-1}.
\end{align*}

Since firm conditions are identical, we can assume price symmetry across firms so $p_{j, t} = p_{j', t}$ for $j \neq j'$. Using the price aggregator, this gets
\begin{equation*}
    P_t = \left(\int_0^1 p_{j, t}^{1 - \psi_t} dj \right)^\frac{1}{1 - \psi_t} = \left(p_{j, t}^{1 - \psi_t} \right)^\frac{1}{1 - \psi_t} = p_j.
\end{equation*}
Additionally, since our perturbation method linearizes the system around the steady state, we can ignore the part that's zero in a first order approximation. Finally, rearranging the system yields the Philips Curve
\begin{equation*}
    \left(\frac{\pi_t}{\overline{\pi}} - 1\right) = \kappa \left(\frac{W_t}{A_t} - \frac{1}{\psi_t}\right) + R_{t+1} \frac{Y_{t+1}}{Y_t} \left(\frac{\pi_{t+1}}{\overline{\pi}} - 1\right) 
\end{equation*}

\subsection{Aggregation}

In the model, firm conditions are perfectly symmetrical. Therefore, for $j \neq j'$ we can assume
\begin{align*}
    y_{j, t} &= y_{j', t} \\
    n_{j, t} &= n_{j', t} \\
    d_{j, t} &= d_{j', t} \\
    m_{j, t} &= m_{j', t}
\end{align*}
Using the aggregators for each variable this gets
\begin{align*}
    Y_t &= \left( \int_0^1 y_{j, t}^\frac{\psi_t - 1}{\psi_t} dj \right)^\frac{\psi_t}{\psi_t - 1} = \left( y_{j, t}^\frac{\psi_t - 1}{\psi_t} \right)^\frac{\psi_t}{\psi_t - 1} = y_{j, t} \\
    N_t &= \int_0^1 n_{j, t} dj = n_{j, t} \\
    D_t &= \int_0^1 d_{j, t} dj = d_{j, t} \\
    M_t &= \int_0^1 m_{j, t} dj = m_{j, t}.
\end{align*}

Then, integrating across the production function gets
\begin{equation*}
    Y_t = \int_0^1 y_{j, t} dj = \int_0^1 A_t n_{j, t} dj = A_t N_t,
\end{equation*}
integrating across the dividend expression gets
\begin{equation*}
    D_t = \int_0^1 d_{j, t} dj = \int_0^1 \left( \frac{p_{j, t}}{P_t} y_{j, t} - W_t n_{j, t} - m_{j, t} \right) dj = Y_t - W_t N_t - M_t,
\end{equation*}
and integrating across the adjustment cost expression gets
\begin{equation*}
    M_t = \int_0^1 m_{j, t} dj = \int_0^1 \frac{\psi_t}{\psi_t - 1}  \frac{1}{2 \kappa} \left(\frac{p_{j, t}}{\overline{\pi} p_{j, t - 1}} - 1\right)^2 y_{j, t} dj = \frac{\psi_t}{\psi_t - 1} \frac{1}{2 \kappa} \left( \frac{\pi_t}{\overline{\pi}} - 1 \right)^2 Y_t.
\end{equation*}


\subsection{Characterization}

The model is characterized by the household decision rules
\begin{align*}
    b_{t} (b_{i, t-1}, z_{i, t}) + c_{t} (b_{i, t-1}, z_{i, t}) &= R_t b_{i, t-1} + W_t z_{i, t} \ell_{t} (b_{i, t-1}, z_{i, t}) + D_t + \eta_t - \tau_t^L z_{i, t}^{\tau_t^P} \\
    c_{t} (b_{i, t-1}, z_{i, t})^{-\gamma} &= \beta \E R_{t + 1} c_{t + 1} (b_{i, t-1}, z_{i, t}) \\
    c_{t} (b_{i, t-1}, z_{i, t})^{-\gamma} &= \frac{\phi}{W_t z_{i, t}} \ell_{t} (b_{i, t-1}, z_{i, t}),
\end{align*}
distributional movement condition
\begin{equation*}
    \Gamma_{t + 1} (b', z') = \int_{\{(b, z) : b_t(b, z) = b'\}} \Pr (z' | z) d \Gamma_t (b, z),
\end{equation*}
aggregate equations
\begin{align*}
    Y_t &= A_t N_t \\
    M_t &= \frac{\psi_t}{\psi_t - 1} \frac{1}{2 \kappa} \left( \frac{\pi_t}{\overline{\pi}} - 1 \right)^2 Y_t \\
    \kappa \frac{\pi_t}{\overline{\pi}} \left( \frac{\pi_t}{\overline{\pi}} - 1 \right) &= 1 - \psi_t + \frac{W_t}{A_t} \psi_t + \kappa \E R_{t + 1}^{-1} \frac{Y_{t + 1}}{Y_t} \frac{\pi_{t + 1}}{\overline{\pi}} \left(\frac{\pi_{t + 1}}{\overline{\pi}} - 1 \right) \\
    D_t &= Y_t - W_t N_t - M_t \\
    G_t &= g_t Y_t \\
    B_t &= (\rho_B + R_t - 1) B_{t - 1} + (2 - \rho_B - \overline{R}) \overline{B} + \eta_t - \overline{\eta} + G_t - \overline{G} \\
    R_t B_{t - 1} + G_t + \eta_t &= \tau_t^L \int z d \Gamma_t^Z (z) + B_t \\
    I_t &= \overline{I} \left(\frac{\pi_t}{\overline{\pi}}\right)^{\omega_\pi} \left(\frac{Y_t}{\overline{Y}}\right)^{\omega_Y} \xi_t \\
    R_t &= \frac{I_{t - 1}}{\pi_t},
\end{align*}
and market clearing conditions
\begin{align*}
    B_t &= \int b_t (b, z) d \Gamma_t (b, z) \\
    N_t &= \int z \ell_z (b, z) d \Gamma_t (b, z)
\end{align*}
where the goods market clears by Walras's Law.
